[FTY::DEFBYTE] Make the size input a keyword argument.
This is more consistent with other FTY macros.

books/kestrel/utilities/fixbytes/defbytelist-tests.lisp
@@ -19,21 +19,21 @@
 ; test successful calls with default options:
 
 (must-succeed*
- (fty::defbyte ubyte8 8)
+ (fty::defbyte ubyte8 :size 8)
  (fty::defbytelist ubyte8-list ubyte8)
  (assert! (function-symbolp 'ubyte8-list-p (w state)))
  (assert! (function-symbolp 'ubyte8-list-fix$inline (w state)))
  (assert! (function-symbolp 'ubyte8-list-equiv$inline (w state))))
 
 (must-succeed*
- (fty::defbyte word 16)
+ (fty::defbyte word :size 16)
  (fty::defbytelist word-list word)
  (assert! (function-symbolp 'word-list-p (w state)))
  (assert! (function-symbolp 'word-list-fix$inline (w state)))
  (assert! (function-symbolp 'word-list-equiv$inline (w state))))
 
 (must-succeed*
- (fty::defbyte sbyte1 1 :signed t)
+ (fty::defbyte sbyte1 :size 1 :signed t)
  (fty::defbytelist sbyte1-list sbyte1)
  (assert! (function-symbolp 'sbyte1-list-p (w state)))
  (assert! (function-symbolp 'sbyte1-list-fix$inline (w state)))
@@ -41,7 +41,7 @@
 
 (must-succeed*
  (defconst *size* 100)
- (fty::defbyte ubyte100 *size*)
+ (fty::defbyte ubyte100 :size *size*)
  (fty::defbytelist ubyte100-list ubyte100)
  (assert! (function-symbolp 'ubyte100-list-p (w state)))
  (assert! (function-symbolp 'ubyte100-list-fix$inline (w state)))
@@ -49,7 +49,7 @@
 
 (must-succeed*
  (define size () 50)
- (fty::defbyte mybyte (size))
+ (fty::defbyte mybyte :size (size))
  (fty::defbytelist mybyte-list mybyte)
  (assert! (function-symbolp 'mybyte-list-p (w state)))
  (assert! (function-symbolp 'mybyte-list-fix$inline (w state)))
@@ -60,7 +60,7 @@
    (((size) => *))
    (local (defun size () 2))
    (defthm posp-of-size (posp (size))))
- (fty::defbyte mybyte (size))
+ (fty::defbyte mybyte :size (size))
  (fty::defbytelist mybyte-list mybyte)
  (assert! (function-symbolp 'mybyte-list-p (w state)))
  (assert! (function-symbolp 'mybyte-list-fix$inline (w state)))
@@ -71,11 +71,11 @@
 ; test the TYPE input:
 
 (must-succeed*
- (fty::defbyte ubyte4 4)
+ (fty::defbyte ubyte4 :size 4)
  (must-fail (fty::defbytelist #\A ubyte4)))
 
 (must-succeed*
- (fty::defbyte ubyte4 4)
+ (fty::defbyte ubyte4 :size 4)
  (fty::defbytelist nibbles ubyte4)
  (assert! (function-symbolp 'nibbles-p (w state)))
  (assert! (function-symbolp 'nibbles-fix$inline (w state)))
@@ -94,11 +94,11 @@
 (must-fail (fty::defbytelist byte-list nat))
 
 (must-succeed*
- (fty::defbyte mybyte 8)
+ (fty::defbyte mybyte :size 8)
  (must-fail (fty::defbytelist mybyte-list mybyt)))
 
 (must-succeed*
- (fty::defbyte mybyte 5)
+ (fty::defbyte mybyte :size 5)
  (fty::defbytelist mybyte-list mybyte)
  (assert! (mybyte-list-p '(0 1 31)))
  (assert! (not (mybyte-list-p '(32)))))
@@ -108,11 +108,11 @@
 ; test the :PRED input:
 
 (must-succeed*
- (fty::defbyte byte 4)
+ (fty::defbyte byte :size 4)
  (must-fail (fty::defbytelist bytes byte :pred 888)))
 
 (must-succeed*
- (fty::defbyte ubyte4 4)
+ (fty::defbyte ubyte4 :size 4)
  (fty::defbytelist ubyte4-list ubyte4 :pred nibblesp)
  (assert! (function-symbolp 'nibblesp (w state)))
  (assert! (function-symbolp 'ubyte4-list-fix$inline (w state)))
@@ -123,11 +123,11 @@
 ; test the :FIX input:
 
 (must-succeed*
- (fty::defbyte byte 4)
+ (fty::defbyte byte :size 4)
  (must-fail (fty::defbytelist bytes byte :fix #c(1 2))))
 
 (must-succeed*
- (fty::defbyte ubyte4 4)
+ (fty::defbyte ubyte4 :size 4)
  (fty::defbytelist ubyte4-list ubyte4 :fix nibfix)
  (assert! (function-symbolp 'ubyte4-list-p (w state)))
  (assert! (function-symbolp 'nibfix$inline (w state)))
@@ -138,11 +138,11 @@
 ; test the :EQUIV input:
 
 (must-succeed*
- (fty::defbyte ubyte4 4)
+ (fty::defbyte ubyte4 :size 4)
  (must-fail (fty::defbytelist ubyte4-list ubyte4 :equiv (1 1 1))))
 
 (must-succeed*
- (fty::defbyte ubyte4 4)
+ (fty::defbyte ubyte4 :size 4)
  (fty::defbytelist ubyte4-list ubyte4 :equiv nibeq)
  (assert! (function-symbolp 'ubyte4-list-p (w state)))
  (assert! (function-symbolp 'ubyte4-list-fix$inline (w state)))
@@ -153,15 +153,15 @@
 ; test the :PARENTS input:
 
 (must-succeed*
- (fty::defbyte byte 4)
+ (fty::defbyte byte :size 4)
  (must-fail (fty::defbytelist byte-list byte :parents one)))
 
 (must-succeed*
- (fty::defbyte byte 4)
+ (fty::defbyte byte :size 4)
  (fty::defbytelist byte-list byte :parents nil))
 
 (must-succeed*
- (fty::defbyte byte 4)
+ (fty::defbyte byte :size 4)
  (fty::defbytelist byte-list byte :parents (this that)))
 
 ;;;;;;;;;;;;;;;;;;;;;;;;;;;;;;;;;;;;;;;;;;;;;;;;;;;;;;;;;;;;;;;;;;;;;;;;;;;;;;;;
@@ -169,15 +169,15 @@
 ; test the :SHORT input:
 
 (must-succeed*
- (fty::defbyte byte 4)
+ (fty::defbyte byte :size 4)
  (must-fail (fty::defbytelist bytes byte :short #\s)))
 
 (must-succeed*
- (fty::defbyte byte 4)
+ (fty::defbyte byte :size 4)
  (fty::defbytelist bytes byte :short "Short doc."))
 
 (must-succeed*
- (fty::defbyte byte 4)
+ (fty::defbyte byte :size 4)
  (fty::defbytelist bytes byte :short (concatenate 'string "Short" " " "doc.")))
 
 ;;;;;;;;;;;;;;;;;;;;;;;;;;;;;;;;;;;;;;;;;;;;;;;;;;;;;;;;;;;;;;;;;;;;;;;;;;;;;;;;
@@ -185,13 +185,13 @@
 ; test the :LONG input:
 
 (must-succeed*
- (fty::defbyte byte 4)
+ (fty::defbyte byte :size 4)
  (must-fail (fty::defbytelist bytes byte :long (#\t #\o #\p #\i #\c))))
 
 (must-succeed*
- (fty::defbyte byte 4)
+ (fty::defbyte byte :size 4)
  (fty::defbytelist bytes byte :long "<p>More doc.</p>"))
 
 (must-succeed*
- (fty::defbyte byte 4)
+ (fty::defbyte byte :size 4)
  (fty::defbytelist bytes byte :long (xdoc::toppstring "More doc.")))
